Prove strong normalization

Phoas.v
@@ -1,769 +1,311 @@
 Require Import Bool.
 Require Import Coqprime.elliptic.ZEll.
-
-(** For F_p *)
 Require Import Coqprime.elliptic.ZEll.
 Require Import Coq.ZArith.Znumtheory.
 Require Import Coq.ZArith.BinInt.
 
 From STLCZK Require Import GaloisField.
+From STLCZK Require Import Ltac.
 From Coq Require Import Vectors.VectorDef.
 From Coq Require Import Init.Nat.
+From Coq  Require Import Program.Equality.
 
 Set Implicit Arguments.
+Set Maximal Implicit Insertion.
 
-(** Use the same reified type for the whole development *)
-Inductive type : Type :=
-| TBool: type
-| TInt: type
-| TArrow : type -> type -> type.
-
-Module Stlc_Phoas(Import PF: GaloisField.GaloisField).
+Module Stlc(Import PF: GaloisField.GaloisField).
   Import PF.
 
-  Section vars.
-  Variable var : type -> Type.
+  (** Use the same reified type for the whole development *)
+  Inductive type : Type :=
+  | TBool: type
+  | TNum: type
+  | TArrow : type -> type -> type.
 
-  Inductive fop : Set := 
-  | op_add : fop
-  | op_sub : fop
-  | op_mul : fop.
+  Declare Custom Entry stlc_ty.
+  Notation "<{{ e }}>" := e (e custom stlc_ty at level 99).
+  Notation "( x )" := x (in custom stlc_ty, x at level 99).
+  Notation "x" := x (in custom stlc_ty at level 0, x constr at level 0).  
+  Notation "S -> T" := (TArrow S T) (in custom stlc_ty at level 2, right associativity).
+  Notation "'Num'" := TNum (in custom stlc_ty at level 0).
+  Notation "'Bool'" := TBool (in custom stlc_ty at level 0).
 
-  Inductive bop: Set :=
-  | op_and : bop
-  | op_or : bop.
-  
-  Inductive term : type -> Type :=
-  | ECField : Fp -> term TInt
-  | ECBool: bool -> term TBool
-         
-  | EVar : forall t,
-      var t
-      -> term t
-             
-  | EApp : forall t1 t2,
-      term (TArrow t1 t2)
-      -> term t1
-      -> term t2
-  | EAbs : forall t1 t2,
-      (var t1 -> term t2)
-      -> term (TArrow t1 t2)
-
-  (** Control flow *)
-  | EIf: forall t, term TBool ->
-         term t ->
-         term t ->
-         term t
-
-  (** Prim ops *)
-  | EFop: fop ->
-          term TInt ->
-          term TInt ->
-          term TInt
-  | EBop: bop ->
-          term TBool ->
-          term TBool ->
-          term TBool
-  | EFeq: term TInt ->
-          term TInt ->
-          term TBool
-  | ENot: term TBool ->
-          term TBool.
-End vars.
-  
-Arguments EVar [var t].
-Arguments ECField {var}.
-Arguments ECBool {var}.
-Arguments EApp [var t1 t2].
-Arguments EAbs [var t1 t2].
-Arguments EIf [var t].
-Arguments EFop {var}.
-Arguments EBop {var}.
-Arguments EFeq {var}.
-Arguments ENot {var}.
-
-Fixpoint typeDenote (t : type) : Set :=
-  match t with
-  | TBool => bool
-  | TInt => Fp
-  | TArrow t1 t2 => typeDenote t1 -> typeDenote t2
-  end.
-
-Fixpoint termDenote t (e : term typeDenote t) {struct e} : typeDenote t :=
-  match e in (term _ t) return (typeDenote t) with
-    | EVar v => v
-
-    | ECBool t => t
-    | ECField f => f
-
-    | EApp e1 e2 => (termDenote e1) (termDenote e2)
-    | EAbs e' => fun x => termDenote (e' x)
-
-    | EIf c e1 e2 => if (termDenote c) then (termDenote e1) else (termDenote e2)
-
-    | EFop op_add e1 e2 => pkplus (termDenote e1) (termDenote e2)
-    | EFop op_sub e1 e2 => pksub (termDenote e1) (termDenote e2)
-    | EFop op_mul e1 e2 => pkmul (termDenote e1) (termDenote e2)
-    | EBop op_and e1 e2 => andb (termDenote e1) (termDenote e2)
-    | EBop op_or e1 e2 => orb (termDenote e1) (termDenote e2)
-    | EFeq e1 e2 => if eq_field (termDenote e1) (termDenote e2) then true else false
-    | ENot e1 => negb (termDenote e1)
-  end.
-End Stlc_Phoas.
-
-Module DanvyOriginal.
-
-  Definition Int := nat.
-
-  (** The forbidden flag *)
-  Unset Positivity Checking.
-
-  Inductive Term: Type :=
-  | INT: Int -> Term 
-  | ADD: Term -> Term -> Term
-  | APP: Term -> Term -> Term
-  | LAM: (Term -> Term) -> Term.
-
-   Inductive Exp (t: Type) :=
-  | EXP: Term -> Exp t.
-
-  Arguments EXP {t}.
-  Definition int(i: Int): Exp Int :=
-    EXP (INT i).
-  
-  Definition add(a b: Exp Int): Exp Int :=
-    match a, b with
-    | EXP e1, EXP e2 => EXP (ADD e1 e2)
-    end.
-  
-  Definition app a b (f: Exp (a -> b))(o: Exp a) : Exp b :=
-    match f, o with
-    | EXP e1, EXP e2 => EXP (APP e1 e2)
-    end.
-
-  Definition lam a b (f: Exp a -> Exp b): Exp (a -> b) :=
-    EXP (LAM (fun (x: Term) => match f (EXP x) with
-                  | EXP b => b
-                            end)).
-   Definition coerce a (e: Exp (Exp a)): Exp a :=
-    match e with
-    | EXP b => EXP b
-    end.
-
-  Definition uncoerce a (e: Exp a): Exp (Exp a) :=
-    match e with
-    | EXP b => EXP b
-    end.
-      
-  Class Nbe a := {
-    reify: a -> Term;
-    reflect: Term-> a
-                }.
-
-  Instance Nbe_lam a b {na: Nbe a} {nb: Nbe b}: Nbe (a -> b) := {
-    reify v := 
-      LAM (fun x => reify (v (reflect x)));
-    reflect e :=
-      fun x => reflect (APP e (reify x))
-                                                              }.
-
-  Unset Positivity Checking.
-End DanvyOriginal.
-
-Module DanvyPhoas(Import PF: GaloisField.GaloisField).
-  Import PF.
-  
   Section vars.
     Variable var : type -> Type.
 
     Inductive Term: type -> Type :=
-    | INT: Fp -> Term TInt
-    | BOOL: bool -> Term TBool
-    | ADD: Term TInt -> Term TInt -> Term TInt
-    | APP: forall a b, Term (TArrow a b) -> Term a -> Term b
+    (* Constants *)
+    | NUM: Fp -> Term <{{ Num }}>
+    | BOOL: bool -> Term <{{ Bool }}>
+    (* Finite field arithmetic *)
+    | ADD: Term <{{ Num }}> -> Term <{{ Num }}> -> Term <{{ Num }}>
+    | SUB: Term <{{ Num }}> -> Term <{{ Num }}> -> Term <{{ Num }}>
+    | MUL: Term <{{ Num }}> -> Term <{{ Num }}> -> Term <{{ Num }}>
+    | DIV: Term <{{ Num }}> -> Term <{{ Num }}> -> Term <{{ Num }}>
+    (* Logical formulas *)
+    | EQ: Term <{{ Num }}> -> Term <{{ Num }}> -> Term <{{ Bool }}>
+    | AND: Term <{{ Bool }}> -> Term <{{ Bool }}> -> Term <{{ Bool }}>
+    | OR: Term <{{ Bool }}> -> Term <{{ Bool }}> -> Term <{{ Bool }}>
+    | NOT: Term <{{ Bool }}> -> Term <{{ Bool }}>
+    (* Control flow *)
+    | ITE: forall t, Term <{{ Bool }}> -> Term t -> Term t -> Term t
+    (* Lambda *)
+    | APP: forall a b, Term <{{ a -> b }}> -> Term a -> Term b
     | VAR: forall a, var a -> Term a
-    | LAM: forall a b, (var a -> Term b) -> Term (TArrow a b).
-  
-  Fixpoint typeDenote (t : type) : Set :=
-    match t with
-    | TBool => bool
-    | TInt => Fp
-    | TArrow t1 t2 => typeDenote t1 -> typeDenote t2
-    end.
-
-  Class Nbe (t: type) := {
-    reify: typeDenote t -> Term t;
-    reflect: Term t -> typeDenote t
-                }.
-
-  Instance Nbe_lam {a b: type} {na: Nbe a} {nb: Nbe b}: Nbe (TArrow a b) := {
-    reify v := 
-      LAM (fun x => reify (v (reflect (VAR x))));
-    reflect e :=
-      fun x => reflect (APP e (reify x))
-                                                                   }.
-  End vars.
-
-  Arguments VAR [var a].
-  Arguments INT {var}.
-  Arguments BOOL {var}.
-  Arguments ADD {var}.
-  Arguments APP [var a b].
-  Arguments LAM [var a b].
-  (** Maximally insert types in class as well *)
-  Arguments Nbe [var].
-  Arguments Nbe_lam [var a b].
-  
-  Fixpoint termDenote t (e : Term typeDenote t) {struct e} : typeDenote t :=
-    match e in (Term _ t) return (typeDenote t) with
-    | VAR v => v
-    | INT f => f
-    | BOOL v => v
-    | ADD f1 f2 => pkplus (termDenote f1) (termDenote f2)
-    | APP e1 e2 => (termDenote e1) (termDenote e2)
-    | LAM e' => fun x => termDenote (e' x)
-    end.
-
-  Instance Nbe_int : Nbe TInt := {
-    reify v := INT v;
-
-    reflect v := termDenote v;
-                                }.
-  Instance Nbe_bool : Nbe TBool := {
-    reify v := BOOL v;
-    
-    reflect v := termDenote v;
-                                }.
-End DanvyPhoas.
-
-Module DanvyPhoasNf(Import PF: GaloisField.GaloisField).
-  Import PF.
-
-  Section vars.
-    Variable var : type -> Type.
+    | LAM: forall a b, (var a -> Term b) -> Term <{{ a ->  b }}>.
 
     Fixpoint typeDenote (t : type) : Set :=
       match t with
-      | TBool => bool
-      | TInt => Fp
-      | TArrow t1 t2 => typeDenote t1 -> typeDenote t2
+      | <{{ Bool }}> => bool
+      | <{{ Num }}> => Fp
+      | <{{ t1 -> t2 }}> => typeDenote t1 -> typeDenote t2
       end.
 
-    (** Danvy paper:
-        data NfTerm = COERCE AtTerm | LAM (AtTerm → NfTerm)
-        data AtTerm = APP AtTerm NfTerm
-      + PHOAS
-     *)
-    Inductive NfTerm: type -> Type :=
-    | NCOERCE: forall t, AtTerm t -> NfTerm t
-    | LAM: forall a b, (var a -> NfTerm b) -> NfTerm (TArrow a b)
-    with AtTerm: type -> Type :=
-    | VAR: forall a, var a -> AtTerm a (** Is var correctly an AtTerm ? *)
-    | APP: forall a b, AtTerm (TArrow a b) -> NfTerm a -> AtTerm b
-    | PCOERCE: forall t, PrTerm t -> AtTerm t
-    | ADD: AtTerm TInt -> AtTerm TInt -> AtTerm TInt
-    with PrTerm: type -> Type :=
-    | INT: Fp -> PrTerm TInt
-    | BOOL: bool -> PrTerm TBool.
-
+    (* Normalization via reify/reflect Danvy et al. *)
     Class Nbe (t: type) := {
-      reify: typeDenote t -> NfTerm t;
-      reflect: AtTerm t -> typeDenote t
+      reify: typeDenote t -> Term t;
+      reflect: Term t -> typeDenote t
                           }.
 
-    Instance Nbe_lam {a b: type} {na: Nbe a} {nb: Nbe b}: Nbe (TArrow a b) := {
+    Instance Nbe_lam {a b: type} `{Nbe a} `{Nbe b}: Nbe <{{ a -> b }}> := {
       reify v := 
         LAM (fun x => reify (v (reflect (VAR x))));
       reflect e :=
         fun x => reflect (APP e (reify x))
-                                                                   }.
+                                                                        }.
   End vars.
 
   Arguments VAR [var a].
-  Arguments INT {var}.
+  Arguments NUM {var}.
   Arguments BOOL {var}.
   Arguments ADD {var}.
-  Arguments NCOERCE [var t].
+  Arguments SUB {var}.
+  Arguments MUL {var}.
+  Arguments DIV {var}.
+  Arguments EQ {var}.
+  Arguments AND {var}.
+  Arguments OR {var}.
   Arguments APP [var a b].
-  Arguments PCOERCE [var t].
   Arguments LAM [var a b].
-  (** Maximally insert types in class as well *)
-  Arguments Nbe [var].
-  Arguments Nbe_lam [var a b].
+  (** Maximally insert types in class *)
+  Arguments Nbe {var}.
+  Arguments Nbe_lam {var} {a} {b}.
+  Arguments reify {var} {t}.
+  Arguments reflect {var} {t}.
 
-  (** Danvy's nf and at + primitive terms Int and Bool *)
-  Fixpoint nfTermDenote t (e : NfTerm typeDenote t) {struct e} : typeDenote t :=
-    match e in (NfTerm _ t) return (typeDenote t) with
-    | NCOERCE a => atTermDenote a
-    | LAM f => fun x => nfTermDenote (f x)
-    end
-  with atTermDenote t (e: AtTerm typeDenote t) {struct e}: typeDenote t :=
-    match e in (AtTerm _ t) return (typeDenote t) with
-    | APP e1 e2 => (atTermDenote e1) (nfTermDenote e2)
-    | VAR v => v
-    | PCOERCE p => prTermDenote p
-    | ADD f1 f2 => pkplus (atTermDenote f1) (atTermDenote f2)
-    end
-  with prTermDenote t (e: PrTerm typeDenote t) {struct e}: typeDenote t :=
-    match e in (PrTerm _ t) return (typeDenote t) with
-    | INT v => v
-    | BOOL v => v
-    end.
-
-  Instance Nbe_int : Nbe TInt := {
-    reify v := NCOERCE (PCOERCE (INT v));
-
-    reflect v := atTermDenote v;
-                                }.
-
-  Instance Nbe_bool : Nbe TBool := {
-    reify v := NCOERCE (PCOERCE (BOOL v));
-    
-    reflect v := atTermDenote v;
-                                }.
-End DanvyPhoasNf.
-
-(** ScratchPAD *)         
-Fixpoint termDenoteReify t (x : typeDenote t) : term typeDenote t :=
-  match t return (_ = _ -> term typeDenote t) with
-  | TBool => (fun _: t = x => ECBool x)
-  | TField => ECField x
-  | TArrow t1 t2 => EAbs (fun v => x (termDenote t1 (EVar v)))
-  end.
-
-Definition Term t := forall var, term var t.
-Definition TermDenote t (e : Term t) := termDenote (e _).
-
-Fixpoint closed_value(t: type): Term t :=
-  match t with
-  | TField => fun _ => ECField (0:%p)
-  | TBool => fun _ => ECBool true
-  | TArrow _ t2 => fun _ => EAbs (fun _ => @closed_value t2 _)
-  end.
-
-Definition input_type(t: type): type :=
-  match t with
-  | TArrow t1 t2 => t1
-  | _ => t
-  end.
-
-Fixpoint closed t (e: term _ t): bool :=
-  match e with
-  | EVar v => true
-  | ECBool _ => false
-  | ECField _ => false
-  | EApp e1 e2 => andb (closed e1) (closed e2)
-  | EIf c e1 e2 => andb (closed c) (andb (closed e1) (closed e2))
-  | EFop _ e1 e2 => andb (closed e1) (closed e2)
-  | EBop _ e1 e2 => andb (closed e1) (closed e2)
-  | EFeq e1 e2 => andb (closed e1) (closed e2)
-  | ENot e => closed e
-  | EAbs e' => closed (e' (closed_value ))
-  end.
-
-Definition value(t: type): Term t -> Prop :=
-  match t with
-  | TField => fun u => exists f: Fp, forall v, u v = ECField f
-  | TBool => fun u => exists b: bool, forall v, u v = ECBool b
-  | TArrow t1 t2 => fun u => forall v, exists f: v t1 -> term v t2, u v = EAbs f
-  end.
-
-Fixpoint computation(t: type): Term t -> Prop :=
-  fun m => exists v, termDenote m = v
-
-                    
-
-Inductive fot: type -> Prop :=
-| FotB: fot TBool
-| FotF: fot TField.
-
-Definition fo_term(t: type) := { e: Term t | fot t }.
-
-End Stlc_Phoas.
-
-Module Stlc(Import PF: GaloisField.GaloisField).
-  Import PF.
-  Include Stlc_Phoas PF.
-  
-  Declare Custom Entry stlc_ty.
   Declare Custom Entry stlc.
-  
-  Notation "'fp' n" := (ECField n) (in custom stlc at level 0).
+  Notation "'fp' n" := (NUM n) (in custom stlc at level 0).
   Notation "'true'"  := true (at level 1).
-  Notation "'true'" := (ECBool true) (in custom stlc at level 0).
+  Notation "'true'" := (BOOL true) (in custom stlc at level 0).
   Notation "'false'"  := false (at level 1).
-  Notation "'false'" := (ECBool false) (in custom stlc at level 0).
+  Notation "'false'" := (BOOL false) (in custom stlc at level 0).
   Notation "<{ e }>" := e (e custom stlc at level 99).
-  Notation "<{{ e }}>" := e (e custom stlc_ty at level 99).
   Notation "( x )" := x (in custom stlc, x at level 99).
-  Notation "( x )" := x (in custom stlc_ty, x at level 99).
   Notation "x" := x (in custom stlc at level 0, x constr at level 0).
-  Notation "x" := x (in custom stlc_ty at level 0, x constr at level 0).  
-  Notation "x y" := (EApp x y) (in custom stlc at level 1, left associativity).
-  
+  Notation "x y" := (APP x y) (in custom stlc at level 1, left associativity).
   Notation "\ x , y" :=
-    (EAbs (fun x => y)) (in custom stlc at level 90,
-                 y custom stlc at level 80,
-                 left associativity).
+    (LAM (fun x => y)) (in custom stlc at level 90,
+                        x constr,
+                        y custom stlc at level 80,
+                        left associativity).
   Notation "\_ , y" :=
-    (EAbs (fun _ => y)) (in custom stlc at level 90,
-                 y custom stlc at level 80,
-                 left associativity).
-  
-  Notation "# n" := (EVar n) (in custom stlc at level 0).
-  Notation "{ x }" := x (in custom stlc at level 1, x constr).
-  Notation "S -> T" := (TArrow S T) (in custom stlc_ty at level 2, right associativity).
-  Notation "'Field'" := TField (in custom stlc_ty at level 0).
-  Notation "'Bool'" := TBool (in custom stlc_ty at level 0).
-  
-  Notation "x + y" := (EFop op_add x y) (in custom stlc at level 2,
+    (LAM (fun _ => y)) (in custom stlc at level 90,
+                        y custom stlc at level 80,
+                        left associativity).
+  Notation "# n" := (VAR n) (in custom stlc at level 0).
+  Notation "{ x }" := x (in custom stlc at level 1, x constr).  
+  Notation "x + y" := (ADD x y) (in custom stlc at level 2,
                                             left associativity).
-  Notation "x - y" := (EFop op_sub x y) (in custom stlc at level 2,
+  Notation "x - y" := (SUB x y) (in custom stlc at level 2,
                                             left associativity).
-  Notation "x * y" := (EFop op_mul x y) (in custom stlc at level 1,
+  Notation "x * y" := (MUL x y) (in custom stlc at level 1,
                                             left associativity).
-  Notation "x && y" := (EBop op_and x y) (in custom stlc at level 4,
+  Notation "x && y" := (AND x y) (in custom stlc at level 4,
                                              left associativity).
-  Notation "x || y" := (EBop op_or x  y) (in custom stlc at level 4,
+  Notation "x || y" := (OR x y) (in custom stlc at level 4,
                                              left associativity).
-  Notation "x == y" := (EFeq x y) (in custom stlc at level 3,
+  Notation "x == y" := (EQ x y) (in custom stlc at level 3,
                                       left associativity).
-  Notation "! x " := (ENot x) (in custom stlc at level 3).
-
+  Notation "! x " := (NOT x) (in custom stlc at level 3).
   Notation "'if' x 'then' y 'else' z" :=
-    (EIf x y z) (in custom stlc at level 89,
+    (ITE x y z) (in custom stlc at level 89,
                     x custom stlc at level 99,
                     y custom stlc at level 99,
                     z custom stlc at level 99,
                     left associativity).
-
-Definition fals : Term <{{ Bool }}> := fun _ => <{ false }>.
-Eval compute in TermDenote fals.
-
-Definition tru : Term <{{ Bool }}> := fun _ => <{ true }>.
-Eval compute in TermDenote tru.
-
-Definition ident : Term <{{ Bool -> Bool }}> := fun _ => <{ \x , #x }>.
-Eval compute in (TermDenote ident).
-
-Definition fals_again : Term Bool := fun _ => ident _ @ fals _.
-Eval compute in TermDenote fals_again.
-
-Definition first : Term (Bool --> Bool --> Bool) := fun _ => \x, \y, #x.
-Eval compute in TermDenote first.
-
-Definition second : Term (Bool --> Bool --> Bool) := fun _ => \x, \y, #y.
-Eval compute in TermDenote second.
-
-Definition test_first : Term Bool := fun _ => first _ @ fals _ @ tru _.
-Eval compute in TermDenote test_first.
-
-Definition test_second : Term Bool := fun _ => second _ @ fals _ @ tru _.
-Eval compute in TermDenote test_second.
-
-Definition app : Term ((Bool --> Bool) --> Bool --> Bool) :=
-  fun _ => \f, \x, #f @ #x.
-Eval compute in TermDenote app.
-
-Definition fals_again2 : Term Bool := fun _ => app _ @ ident _ @ fals _.
-Eval compute in TermDenote fals_again2.        
-
-Section normalize.
-  Definition fo: Type -> Prop :=
-    | FoBool bool_scope
-  Fixpoint normalize a Term a -> 
-
-(** CPS *)
-Inductive ptype : Type :=
-| PBool : ptype
-| PCont : ptype -> ptype
-| PUnit : ptype
-| PProd : ptype -> ptype -> ptype.
-
-Notation "'Bool'" := PBool : cps_scope.
-Notation "t --->" := (PCont t) (at level 61) : cps_scope.
-Notation "'Unit'" := PUnit : cps_scope.
-Infix "**" := PProd (right associativity, at level 60) : cps_scope.
-
-Bind Scope cps_scope with ptype.
-Delimit Scope cps_scope with cps.
-
-Section vars.
-  Variable var : ptype -> Type.
-
-  Variable result : ptype.
-
-  Inductive pterm : Type :=
-  | PHalt :
-    var result
-    -> pterm
-  | PApp : forall t,
-    var (t --->)
-    -> var t
-    -> pterm
-  | PBind : forall t,
-    pprimop t
-    -> (var t -> pterm)
-    -> pterm
-
-  with pprimop : ptype -> Type :=
-  | PVar : forall t,
-    var t
-    -> pprimop t
-    
-  | PTrue : pprimop Bool
-  | PFalse : pprimop Bool
-    
-  | PAbs : forall t,
-    (var t -> pterm)
-    -> pprimop (t --->)
-
-  | PPair : forall t1 t2,
-    var t1
-    -> var t2
-    -> pprimop (t1 ** t2)
-  | PFst : forall t1 t2,
-    var (t1 ** t2)
-    -> pprimop t1
-  | PSnd : forall t1 t2,
-    var (t1 ** t2)
-    -> pprimop t2.
-  Check pterm_ind.
-End vars.
-
-Arguments PHalt [var result].
-Arguments PApp [var result t].
-Arguments PBind [var result t].
-
-Arguments PVar [var result t].
-Arguments PTrue {var result}.
-Arguments PFalse {var result}.
-Arguments PAbs [var result t].
-Arguments PPair [var result t1 t2].
-Arguments PFst [var result t1 t2].
-Arguments PSnd [var result t1 t2].
-
-Notation "'Halt' x" := (PHalt x) (no associativity, at level 75) : cps_scope.
-Infix "@@" := PApp (no associativity, at level 75) : cps_scope.
-Notation "x <- p ; e" := (PBind p (fun x => e))
-  (right associativity, at level 76, p at next level) : cps_scope.
-Notation "! <- p ; e" := (PBind p (fun _ => e))
-  (right associativity, at level 76, p at next level) : cps_scope.
-
-Notation "# v" := (PVar v) (at level 70) : cps_scope.
-
-Notation "'Tru'" := PTrue : cps_scope.
-Notation "'Fals'" := PFalse : cps_scope.
-
-Notation "\ x , e" := (PAbs (fun x => e)) (at level 78) : cps_scope.
-Notation "\ ! , e" := (PAbs (fun _ => e)) (at level 78) : cps_scope.
-
-Notation "[ x1 , x2 ]" := (PPair x1 x2) (at level 73) : cps_scope.
-Notation "#1 x" := (PFst x) (at level 72) : cps_scope.
-Notation "#2 x" := (PSnd x) (at level 72) : cps_scope.
-
-Bind Scope cps_scope with pterm pprimop.
-
-Local Open Scope cps_scope.
-
-Fixpoint ptypeDenote (t : ptype) : Set :=
-  match t with
-    | Bool => bool
-    | t' ---> => ptypeDenote t' -> bool
-    | Unit => unit
-    | t1 ** t2 => (ptypeDenote t1 * ptypeDenote t2)%type
-  end.
-
-Fixpoint ptermDenote result (e : pterm ptypeDenote result) (k : ptypeDenote result -> bool)
-  {struct e} : bool :=
-  match e with
-    | PHalt v => k v
-    | PApp f x => f x
-    | PBind p x => ptermDenote (x (pprimopDenote p k)) k
-  end
-
-with pprimopDenote result t (p : pprimop ptypeDenote result t) (k : ptypeDenote result -> bool)
-  {struct p} : ptypeDenote t :=
-  match p in (pprimop _ _ t) return (ptypeDenote t) with
-    | PVar v => v
-
-    | PTrue => true
-    | PFalse => false
-
-    | PAbs e => fun x => ptermDenote (e x) k
-
-    | PPair v1 v2 => (v1, v2)
-    | PFst v => fst v
-    | PSnd v => snd v
-  end.
-
-Definition Pterm result := forall var, pterm var result.
-Definition Pprimop result t := forall var, pprimop var result t.
-Definition PtermDenote result (e : Pterm result) := ptermDenote (e _).
-Definition PprimopDenote result t (p : Pprimop result t) := pprimopDenote (p _).
-                                                               
-(** * CPS translation *)
-
-(** ** Translating types *)
-
-Fixpoint cpsType (t : type) : ptype :=
-  match t with
-    | Bool => Bool%cps
-    | t1 --> t2 => (cpsType t1 ** (cpsType t2 --->) --->)%cps
-  end%source.
-
-(** ** Translating terms *)
-
-Section splice.
-  Local Open Scope cps_scope.
-
-  Fixpoint splice (var : ptype -> Type) (result1 result2 : ptype) (e1 : pterm var result1) (e2 : var result1 -> pterm var result2) {struct e1} : pterm var result2 :=
-    match e1 with
-      | PHalt v => e2 v
-      | PApp f x => f @@ x
-      | PBind p e' => x <- splicePrim p e2; splice (e' x) e2
-    end
-
-  with splicePrim (var : ptype -> Type) (result1 result2 : ptype) t (p : pprimop var result1 t) (e2 : var result1 -> pterm var result2) {struct p} : pprimop var result2 t :=
-    match p in (pprimop _ _ t) return (pprimop var result2 t) with
-      | PVar v => #v
-
-      | PTrue => Tru
-      | PFalse => Fals
-
-      | PAbs e => \x, splice (e x) e2
-
-      | PPair v1 v2 => [v1, v2]
-
-      | PFst v => #1 v
-      | PSnd v => #2 v
+  
+  Fixpoint termDenote t (e : Term typeDenote t) {struct e} : typeDenote t :=
+    match e in (Term _ t) return (typeDenote t) with
+    | VAR v => v
+    | NUM f => f
+    | BOOL v => v
+    | ADD f1 f2 => pkplus (termDenote f1) (termDenote f2)
+    | SUB f1 f2 => pksub (termDenote f1) (termDenote f2)
+    | MUL f1 f2 => pkmul (termDenote f1) (termDenote f2)
+    | DIV f1 f2 => pkdiv (termDenote f1) (termDenote f2)
+    | EQ f1 f2 => if eq_field (termDenote f1) (termDenote f2) then true else false
+    | ITE c t e => if (termDenote c) then termDenote t else termDenote e
+    | AND b1 b2 => andb (termDenote b1) (termDenote b2)
+    | OR b1 b2 => orb (termDenote b1) (termDenote b2)
+    | NOT b => negb (termDenote b)
+    | APP e1 e2 => (termDenote e1) (termDenote e2)
+    | LAM e' => fun x => termDenote (e' x)
     end.
-End splice.
 
-Notation "x <-- e1 ; e2" := (splice e1 (fun x => e2))
-  (right associativity, at level 76, e1 at next level) : cps_scope.
-Notation "! <-- e1 ; e2" := (splice e1 (fun _ => e2))
-  (right associativity, at level 76, e1 at next level) : cps_scope.
+  Instance Nbe_int : Nbe <{{ Num }}> := {
+    reify v := NUM v;
+    reflect v := termDenote v;
+                                }.
 
-Section cpsTerm.
-  Variable var : ptype -> Type.
+  Instance Nbe_bool : Nbe <{{ Bool }}> := {
+    reify v := BOOL v;
+    reflect v := termDenote v;
+                                  }.
 
-  Notation var' := (fun t => var (cpsType t)).
+  Compute reify _ true.
+  Compute reify (Nbe_lam _ _) (fun x => x).
+  Compute reify (Nbe_lam _ _) (fun x => (fun y => y) true).
+  Compute reflect (Nbe_lam _ _) <{ \_, true }>.
+  Compute reify (Nbe_lam _ _ ) (fun x => (fun y => y) true).
+  Compute reflect (Nbe_lam _ _)
+          (reify (Nbe_lam _ _ ) (fun x => (fun y => y) true)).  
+  Compute reflect (Nbe_lam _ _ )
+          <{ (\x, \y, # x) true }>.
 
-  Local Open Scope cps_scope.
-
-  Fixpoint cpsTerm t (e : term var' t) {struct e} : pterm var (cpsType t) :=
-    match e in (term _ t) return (pterm var (cpsType t)) with
-      | EVar v => PHalt (var := var) v
-
-      | ETrue => x <- Tru; Halt x
-      | EFalse => x <- Fals; Halt x
-
-      | EApp e1 e2 =>
-        f <-- cpsTerm e1;
-        x <-- cpsTerm e2;
-        k <- \r, PHalt (var := var) r;
-        p <- [x, k];
-        f @@ p
-      | EAbs e' =>
-        f <- PAbs (var := var) (fun p =>
-          x <- #1 p;
-          k <- #2 p;
-          r <-- cpsTerm (e' x);
-          k @@ r);
-        Halt f
+  Fixpoint resolver(t: type): Nbe t :=
+    match t with
+    | <{{ Bool }}> => Nbe_bool
+    | <{{ Num }}> => Nbe_int
+    | <{{ a -> b }}> => Nbe_lam (resolver a) (resolver b)
     end.
-End cpsTerm.
+    
+  Definition normalize {t: type} (e: Term typeDenote t) : Term typeDenote t :=
+    reify (resolver t) (reflect (resolver t) e).
+                                       
+  Inductive fof: type -> Prop :=
+  | fo_bool: fof <{{ Bool }}>
+  | fo_num: fof <{{ Num }}>
+  | fof_bool: forall a,
+      fof <{{ a }}> ->
+      fof <{{ Bool -> a }}>
+  | fof_num: forall a,
+      fof <{{ a }}> ->
+      fof <{{ Num -> a }}>.
 
-Arguments cpsTerm [var t].
-Definition CpsTerm t (E : Term t) : Pterm (cpsType t) := fun _ => cpsTerm (E _).
+  Inductive hnff: forall (t: type), Term typeDenote t -> Prop :=
+  | HNF_bool_ar: forall a f (arg: typeDenote <{{ Bool }}>),
+      @hnff <{{ a }}> (f arg) ->
+      @hnff <{{ Bool -> a }}> (LAM f)
+  | HNF_num_ar: forall a f (arg: typeDenote <{{ Num }}>),
+      @hnff <{{ a }}> (f arg) ->
+      @hnff <{{ Num -> a }}> (LAM f)
+  | HNF_bool: forall e,
+      @hnff <{{ Bool }}> (BOOL e)
+  | HNF_num: forall e,
+      @hnff <{{ Num }}> (NUM e).
 
-(** * Correctness *)
+  (** Provide default witnesses for hnff *)
+  Hint Extern 3 (typeDenote <{{ Bool }}>) => exact (true).
+  Hint Extern 3 (typeDenote <{{ Num }}>) => exact (0:%p).
 
-(**
+  Theorem normalize_correct: forall (t: type) (e: Term typeDenote t),
+      fof t  -> 
+      @hnff t (@normalize t e).
+  Proof with eauto.
+    intros.
+    generalize dependent e.
+    generalize dependent H.
+    induction t; intros; dependent destruction e; cbn; try constructor;
+      invert H; cbn; unshelve (econstructor; eauto)...
+  Defined.
+
+End Stlc.
+
+  (** * Correctness *)
+
+  (**
 pterm_ind
      : forall P : pterm -> Prop,
        (forall v : var result, P (PHalt v)) ->
        (forall (t : ptype) (v : var (t --->)) (v0 : var t), P (PApp v v0)) ->
        (forall (t : ptype) (p : pprimop t) (p0 : var t -> pterm),
         (forall v : var t, P (p0 v)) -> P (PBind p p0)) -> forall p : pterm, P p
-*)
-Scheme pterm_mut := Induction for pterm Sort Prop
-with pprimop_mut := Induction for pprimop Sort Prop.
+   *)
 
-Section splice_correct.
-  Variables result1 result2 : ptype.
 
-  Variable e2 : ptypeDenote result1 -> pterm ptypeDenote result2.  
+  Section splice_correct.
+    Variables result1 result2 : ptype.
 
-  Theorem splice_correct : forall e1 k,
-    ptermDenote (splice e1 e2) k
-    = ptermDenote e1 (fun r => ptermDenote (e2 r) k).
-    apply (pterm_mut
-      (fun e1 => forall k,
+    Variable e2 : ptypeDenote result1 -> pterm ptypeDenote result2.  
+
+    Theorem splice_correct : forall e1 k,
         ptermDenote (splice e1 e2) k
-        = ptermDenote e1 (fun r => ptermDenote (e2 r) k))
-      (fun t p => forall k,
-        pprimopDenote (splicePrim p e2) k
-        = pprimopDenote p (fun r => ptermDenote (e2 r) k))); auto.
-    equation.
-  Qed.
-End splice_correct.
+        = ptermDenote e1 (fun r => ptermDenote (e2 r) k).
+      apply (pterm_mut
+               (fun e1 => forall k,
+                    ptermDenote (splice e1 e2) k
+                    = ptermDenote e1 (fun r => ptermDenote (e2 r) k))
+               (fun t p => forall k,
+                    pprimopDenote (splicePrim p e2) k
+                    = pprimopDenote p (fun r => ptermDenote (e2 r) k))); auto.
+      equation.
+    Qed.
+  End splice_correct.
 
-Fixpoint lr (t : type) : typeDenote t -> ptypeDenote (cpsType t) -> Prop :=
-  match t return (typeDenote t -> ptypeDenote (cpsType t) -> Prop) with
+  Fixpoint lr (t : type) : typeDenote t -> ptypeDenote (cpsType t) -> Prop :=
+    match t return (typeDenote t -> ptypeDenote (cpsType t) -> Prop) with
     | TBool => fun n1 n2 => n1 = n2
     | TArrow t1 t2 => fun f1 f2 =>
-      forall x1 x2, lr _ x1 x2
-        -> forall k, exists r,
-          f2 (x2, k) = k r
-          /\ lr _ (f1 x1) r
-  end.
-
-Lemma cpsTerm_correct : forall G t (e1 : term _ t) (e2 : term _ t),
-  term_equiv G e1 e2
-  -> (forall t v1 v2, In (vars (v1, v2)) G -> lr t v1 v2)
-  -> forall k, exists r,
-    ptermDenote (cpsTerm e2) k = k r
-    /\ lr t (termDenote e1) r.
-  Hint Rewrite splice_correct : ltamer.
-
-  Ltac my_changer :=
-    match goal with
-      [ H : (forall (t : _) (v1 : _) (v2 : _), vars _ = vars _ \/ In _ _ -> _) -> _ |- _ ] =>
-      match typeof H with
-        | ?P -> _ =>
-          assert P; [intros; push_vars; intuition; fail 2
-            | idtac]
-      end
+                       forall x1 x2, lr _ x1 x2
+                                -> forall k, exists r,
+                             f2 (x2, k) = k r
+                             /\ lr _ (f1 x1) r
     end.
 
-  Ltac my_simpler := repeat progress (equation; fold ptypeDenote in *;
-    fold cpsType in *; try my_changer).
+  Lemma cpsTerm_correct : forall G t (e1 : term _ t) (e2 : term _ t),
+      term_equiv G e1 e2
+      -> (forall t v1 v2, In (vars (v1, v2)) G -> lr t v1 v2)
+      -> forall k, exists r,
+            ptermDenote (cpsTerm e2) k = k r
+            /\ lr t (termDenote e1) r.
+    Hint Rewrite splice_correct : ltamer.
 
-  Ltac my_chooser T k :=
-    match T with
+    Ltac my_changer :=
+      match goal with
+        [ H : (forall (t : _) (v1 : _) (v2 : _), vars _ = vars _ \/ In _ _ -> _) -> _ |- _ ] =>
+        match typeof H with
+        | ?P -> _ =>
+          assert P; [intros; push_vars; intuition; fail 2
+                    | idtac]
+        end
+      end.
+
+    Ltac my_simpler := repeat progress (equation; fold ptypeDenote in *;
+                                        fold cpsType in *; try my_changer).
+
+    Ltac my_chooser T k :=
+      match T with
       | bool => fail 1
       | type => fail 1
       | ctxt _ _ => fail 1
       | _ => default_chooser T k
-    end.
+      end.
 
-  induction 1; matching my_simpler my_chooser; eauto.
-Qed.
+    induction 1; matching my_simpler my_chooser; eauto.
+  Qed.
 
-Theorem CpsTerm_correct : forall t (E : Term t),
-  forall k, exists r,
-    PtermDenote (CpsTerm E) k = k r
-    /\ lr t (TermDenote E) r.
-  unfold PtermDenote, TermDenote, CpsTerm; simpl; intros.
-  eapply (cpsTerm_correct (G := nil)); simpl; intuition.
-  apply Term_equiv.
-Qed.
+  Theorem CpsTerm_correct : forall t (E : Term t),
+      forall k, exists r,
+          PtermDenote (CpsTerm E) k = k r
+          /\ lr t (TermDenote E) r.
+    unfold PtermDenote, TermDenote, CpsTerm; simpl; intros.
+    eapply (cpsTerm_correct (G := nil)); simpl; intuition.
+    apply Term_equiv.
+  Qed.
 
-Theorem CpsTerm_correct_bool : forall (E : Term TBool),
-  forall k, PtermDenote (CpsTerm E) k = k (TermDenote E).
-  intros.
-  generalize (CpsTerm_correct E k); firstorder congruence.
-Qed.
+  Theorem CpsTerm_correct_bool : forall (E : Term TBool),
+      forall k, PtermDenote (CpsTerm E) k = k (TermDenote E).
+    intros.
+    generalize (CpsTerm_correct E k); firstorder congruence.
+  Qed.
                                           
